swap$\phantom{^{2}}$T (l : Old.list T)
  : New.list T
:=
  Old.list_rect T
    (fun _ => New.list T)
    New.nil
    (fun$\hspace{-0.1cm}$ t$\hspace{-0.1cm}$ _$\hspace{-0.1cm}$ (IHl: New.list T)$\hspace{-0.1cm}$ =>
      New.cons T t IHl)
    l.

Lemma section:
  $\forall$ T (l : Old.list T),
    swap$^{-1}$ T (swap T l) = l.
Proof.
  intros T l. symmetry.
  induction l as [ |t l0 H].
  - auto.
  - simpl. rewrite $\leftarrow$ H. auto.
Qed.

swap$^{-1}$ T (l : New.list T)
  : Old.list T
:=
  New.list_rect T
    (fun _ => Old.list T)
    (fun$\hspace{-0.1cm}$ t$\hspace{-0.1cm}$ _$\hspace{-0.1cm}$ (IHl: Old.list T)$\hspace{-0.1cm}$ =>
      Old.cons T t IHl)
    Old.nil
    l.

Lemma retraction:
  $\forall$ T (l : New.list T),
    swap T (swap$^{-1}$ T l) = l.
Proof.
  intros T l. symmetry.
  induction l as [t l0 H| ].
  - simpl. rewrite $\leftarrow$ H. auto.
  - auto.
Qed.
